Working on modularizing and expanding proofs.

sel4_artifacts/UxASSeL4/verification/WaypointManagerFunSpec.thy
@@ -1,10 +1,13 @@
 theory WaypointManagerFunSpec imports 
 Main
+Sublist
 begin
   
-locale FindWaypoint =
+locale WaypointManager =
   fixes get_number :: "'w \<Rightarrow> 'id"
-context FindWaypoint begin
+   fixes get_nextwp :: "'w \<Rightarrow> 'id"
+context WaypointManager begin
+
 
 (* FUNSPEC(find_wp): Find a waypoint in a list of waypoints by its number. This is how we 
    notionally expect the find_wp function to work. *)
@@ -31,11 +34,76 @@ proof(induct ws)
 next
   case (Cons a ws)
   then have "None = find_waypoint ws n \<and> get_number a \<noteq> n"
-    by (metis (mono_tags) FindWaypoint.find_waypoint_def find.simps(2) option.distinct(1))
+    by (metis (mono_tags) find_waypoint_def find.simps(2) option.distinct(1))
   then show ?case using Cons by (metis Suc_less_eq gr0_conv_Suc length_Cons not_gr_zero nth_Cons_0 nth_Cons_Suc)
 qed 
 
+(* If a list L1 is a prefix of another L2, that list can be extended by some other list such 
+   that it results L2. *)
+lemma prefix_ident: "prefix ws' ws \<Longrightarrow> \<exists> ws1. ws = ws'@ws1"
+apply (induct ws' arbitrary: ws) using prefix_def by blast+
+  
+(* If a waypoint is found in a prefix L1 the same waypoint will be found in L2. *)
+lemma find_waypoint_ignores_dup_matches:
+  "prefix ws' ws \<Longrightarrow> Some w = find_waypoint ws' n \<Longrightarrow> Some w = find_waypoint ws n"
+proof(induct ws' arbitrary: ws)
+  case Nil
+  then show ?case using find_waypoint_def by auto
+next
+  case (Cons w' ws'')
+  then obtain ws1 where y1:"ws = w' # ws'' @ ws1" by (metis append_Cons prefix_ident Cons)
+  thus ?case using Cons y1 by (metis Sublist.Cons_prefix_Cons find.simps(2) find_waypoint_def)
+qed
+
+lemma find_waypoint_next_is_match:
+assumes a1:"Some w = find_waypoint ws (get_number (ws ! j))"
+and  a2:"None = find_waypoint (take j ws) (get_number (ws ! j))"
+and a3:"j < length ws"
+shows "ws ! j  = w"
+proof -
+  have "prefix (take j ws) ws" using take_is_prefix by blast
+  then have y2:"Some w = find_waypoint (take j ws @ [ws ! j]) (get_number (ws ! j))"
+    by (metis (no_types, lifting) a2  find_waypoint_none_extend_some 
+        a1 a3 find_waypoint_ignores_dup_matches hd_drop_conv_nth take_hd_drop take_is_prefix)
+  thus ?thesis by (metis find_waypoint_none_extend_some a2 option.inject)
+qed
+
+definition waypoints_wf where
+  "waypoints_wf ws \<equiv> (\<forall> w'. List.member ws w' \<longrightarrow> (\<exists> w. Some w = find_waypoint ws (get_nextwp w')))"
+
+  
+fun waypoints_window :: "'w list \<Rightarrow> 'id \<Rightarrow> nat \<Rightarrow> ('w list) option" where
+  "waypoints_window ws i 0 = Some []"
+| "waypoints_window ws i (Suc n) = 
+    (case find_waypoint ws i of
+     Some w \<Rightarrow> 
+       if get_nextwp w = i then Some [w]
+       else 
+        (case waypoints_window ws (get_nextwp w) n of 
+         Some ws \<Rightarrow> Some (w # ws) 
+         | None \<Rightarrow> None)
+    | None \<Rightarrow> None)"
+
+  
+(*
+lemma  "waypoints_wf ws \<Longrightarrow> Some w = find_waypoint ws i \<Longrightarrow> \<exists> win. Some win = waypoints_window ws i len"
+  apply(unfold find_waypoint_def)
+    apply(induct rule:find.induct)
+    
+lemma waypoints_window_lteq_len:"waypoints_wf ws \<Longrightarrow> Some w = find_waypoint ws i \<Longrightarrow> win = waypoints_window ws i len \<Longrightarrow> length win \<le> len"
+  proof(induct len)
+    case 0
+    then show ?case by auto
+  next
+    case (Suc len)
+    then have "length win \<le> len" sledgehammer[z3 e spass]
+    then show ?case
+  qed 
+   apply clarsimp
+*)
     
 end
+  
+
   
 end
