sel4_artifacts/UxASSeL4/verification/FindWPToFunSpec.thy
@@ -3,7 +3,7 @@ theory FindWPToFunSpec imports
 "WaypointManagerFunSpec"
 begin
 
-interpretation FindWaypoint get_waypoint_number done
+interpretation WaypointManager get_waypoint_number nextwaypoint_C done
 
 (* Lift waypoints from a mission command into a list with the same order. *)
 fun lift_waypoints  where
@@ -18,42 +18,19 @@ lemma lift_waypoints_length: "ws = lift_waypoints s mcp n \<Longrightarrow> leng
 lemma lift_waypoints_to_get_waypoint: 
   "ws = lift_waypoints s mcp n \<Longrightarrow> \<forall> k< n.  get_waypoint s mcp k = nth ws k"
 apply(induct n arbitrary: ws) by (auto simp add: less_Suc_eq lift_waypoints_length nth_append)
-
-(* If a list L1 is a prefix of another L2, that list can be extended by some other list such 
-   that it results L2. *)
-lemma prefix_ident: "prefix ws' ws \<Longrightarrow> \<exists> ws1. ws = ws'@ws1"
-apply (induct ws' arbitrary: ws) using prefix_def by blast+
-  
-(* If a waypoint is found in a prefix L1 the same waypoint will be found in L2. *)
-lemma find_waypoint_ignores_dup_matches:
-  "prefix ws' ws \<Longrightarrow> Some w = find_waypoint ws' n \<Longrightarrow> Some w = find_waypoint ws n"
-proof(induct ws' arbitrary: ws)
-  case Nil
-  then show ?case using find_waypoint_def by auto
-next
-  case (Cons w' ws'')
-  then obtain ws1 where y1:"ws = w' # ws'' @ ws1" by (metis append_Cons prefix_ident Cons)
-  thus ?case using Cons y1 by (metis Sublist.Cons_prefix_Cons find.simps(2) find_waypoint_def)
-qed
-
-(* lift_waypoint will create prefixes when s and mcp are fixed and the sizes differ. *)  
-lemma lifted_waypoint_prefixes:" i \<le> j \<Longrightarrow> prefix (lift_waypoints s mcp i) (lift_waypoints s mcp j)"
-apply(induct i) by (metis lift_waypoints.simps(2) prefix_def prefix_order.lift_Suc_mono_le)+    
     
-lemma find_waypoint_next_is_match:
-assumes a1:"Some w = find_waypoint (lift_waypoints s mcp (unat i)) (get_waypoint_number(get_waypoint s mcp (uint j)))"
-and  a2:"None = find_waypoint (lift_waypoints s mcp (unat j)) (get_waypoint_number (get_waypoint s mcp (uint j)))"
-and a3:"j < i"
-shows "get_waypoint s mcp (uint j) = w"
-proof -  
-  have y1:"prefix (lift_waypoints s mcp (unat j) @ [get_waypoint s mcp (uint j)]) (lift_waypoints s mcp (unat i))" 
-    by (metis lifted_waypoint_prefixes  lift_waypoints.simps(2) a3 le_less less_antisym not_less uint_nat word_less_nat_alt )
-  then have y2:"Some (get_waypoint s mcp (uint j)) = find_waypoint (lift_waypoints s mcp (unat j) @ [get_waypoint s mcp (uint j)]) (get_waypoint_number (get_waypoint s mcp (uint j)))"
-    using a2 find_waypoint_none_extend_some by auto
-  show ?thesis using find_waypoint_ignores_dup_matches y1 y2 a1 by (metis option.inject)
-qed 
-
-lemma [simp]: "j < i \<Longrightarrow> int (unat j) = uint j" by (simp add: uint_nat)
+lemma lift_waypoint_to_take:
+  "ws = lift_waypoints s mcp i \<Longrightarrow> j < i \<Longrightarrow> take j ws = lift_waypoints s mcp j"
+proof(induct j arbitrary: ws)
+  case 0
+  then show ?case by auto
+next
+  case (Suc j)
+  then have "take j ws = lift_waypoints s mcp j" by auto
+  thus ?case using Suc
+    by (metis Suc_lessD lift_waypoints.simps(2) lift_waypoints_length lift_waypoints_to_get_waypoint 
+        take_Suc_conv_app_nth)
+qed
   
 lemma find_waypoint_extend_failure:
   assumes a1:"None = find_waypoint (lift_waypoints s mcp (unat (j::32 word))) i"
@@ -68,6 +45,21 @@ proof -
     by (metis Suc_eq_plus1 add.commute less_is_non_zero_p1 unatSuc)
   thus ?thesis using Suc_eq_plus1 y2 by presburger
 qed
+
+lemma find_waypoint_failure_all_neq_number:"ws = lift_waypoints s mcp (unat (get_waypoints_length s mcp)) 
+\<Longrightarrow> None = find_waypoint ws n
+\<Longrightarrow> \<forall>i<unat (get_waypoints_length s mcp). number_C (get_waypoint s mcp (int i)) \<noteq> n"
+  by (metis find_waypoint_failure_not_equal_all_elems 
+      get_waypoint_number_def lift_waypoints_length lift_waypoints_to_get_waypoint)
+
+lemma valid_mission_command[simp]:
+"is_valid_MissionCommand s mcp 
+\<Longrightarrow> j < get_waypoints_length s mcp
+\<Longrightarrow> is_valid_MissionCommand_struct_C s mcp 
+  \<and> is_valid_Waypoint_struct_C s (get_waypoint_ptr s mcp (uint j)) 
+  \<and> is_valid_Waypoint_struct_C'ptr s (get_waypoint_ptr_ptr s mcp (uint j)) 
+  \<and> is_valid_MissionCommand_struct_C s mcp"
+  apply(unfold is_valid_MissionCommand_def) by (metis uint_nat word_less_nat_alt)  
   
 lemma findwp_success:
 "\<lbrace> \<lambda> (s::lifted_globals).
@@ -78,99 +70,82 @@ lemma findwp_success:
 \<lbrace> \<lambda> r s. heap_Waypoint_struct_C s r = w \<and> P s\<rbrace>!"
   apply (unfold LoadCode.MissionCommandUtils.FindWP'_def)
   apply (simp add: skipE_def)
-  apply(subst whileLoopE_add_inv[where M = "\<lambda> (j,s). unat (get_waypoints_length s mcp - j)"
-                                 and I = "\<lambda> j s. P s 
-\<and> is_valid_MissionCommand s mcp
-\<and> Some w = find_waypoint (lift_waypoints s mcp (unat (get_waypoints_length s mcp))) i
-\<and> None = find_waypoint (lift_waypoints s mcp (unat j)) i
-\<and> j \<le> get_waypoints_length s mcp
-"])
-   apply wp
-   apply (simp add: is_valid_MissionCommand_def word_less_nat_alt)+
-     apply rule+
-     apply (intro find_waypoint_next_is_match)
-       using inc_le apply blast+
-     using find_waypoint_extend_failure word_less_nat_alt apply blast
-    apply (metis uint_nat)
-   apply clarsimp
-   apply rule
-    apply (metis find_waypoint_extend_failure get_waypoint_number_def word_less_nat_alt)
-   apply rule
-    using inc_le word_less_nat_alt apply blast
-   apply (metis (no_types, hide_lams) diff_diff_add linorder_not_less measure_unat order_le_less right_minus_eq uint_nat)
-  apply fastforce
- apply wp
- by (simp add: find_waypoint_def is_valid_MissionCommand_def)
-
-lemma find_waypoint_failure_not_equal_all_elems_aux:"None = find_waypoint (lift_waypoints s mcp (unat (get_waypoints_length s mcp))) n 
-\<Longrightarrow> \<forall> i < get_waypoints_length s mcp. number_C (get_waypoint s mcp (int (unat i))) \<noteq> n"
-proof -
-  assume a:"None = find_waypoint (lift_waypoints s mcp (unat (get_waypoints_length s mcp))) n"
-  then obtain ws where y1:"ws = lift_waypoints s mcp (unat (get_waypoints_length s mcp))" and y2:"None = find_waypoint ws n" by auto
-  then have "\<forall>i<length ws. number_C (ws ! i) \<noteq> n" using find_waypoint_failure_not_equal_all_elems y2 by auto
-  then have "\<forall>i<unat (get_waypoints_length s mcp). number_C (ws ! i) \<noteq> n" using lift_waypoints_length[OF y1] by auto
-  then have "\<forall>i<unat (get_waypoints_length s mcp). number_C (get_waypoint s mcp (int i)) \<noteq> n" using lift_waypoints_to_get_waypoint[OF y1] by auto
-  thus ?thesis by (metis of_nat_less_iff uint_nat word_less_def)
-qed
+  apply(subst whileLoopE_add_inv
+        [where 
+          M = "\<lambda> (j,s). unat (get_waypoints_length s mcp - j)"
+          and I = 
+            "\<lambda> j s. P s 
+            \<and> is_valid_MissionCommand s mcp
+            \<and> Some w = find_waypoint (lift_waypoints s mcp (unat (get_waypoints_length s mcp))) i
+            \<and> None = find_waypoint (lift_waypoints s mcp (unat j)) i
+            \<and> j \<le> get_waypoints_length s mcp"
+        ])
+  apply wp
+    apply clarsimp
+    apply rule+
+     apply (metis find_waypoint_next_is_match lift_waypoints_length 
+      lift_waypoints_to_get_waypoint lift_waypoint_to_take uint_nat unat_mono)
+    apply (metis find_waypoint_extend_failure get_waypoint_number_def inc_le) 
+   apply force
+  apply wp
+  using find_waypoint_def is_valid_MissionCommand_def by auto
   
 lemma findwp_failure:
 "\<lbrace> \<lambda> (s::lifted_globals).
-  is_valid_MissionCommand s mcp
-  \<and> None = find_waypoint (lift_waypoints s mcp (unat (get_waypoints_length s mcp))) i
-  \<and> P s\<rbrace>
+  P s
+  \<and> is_valid_MissionCommand s mcp
+  \<and> None = find_waypoint (lift_waypoints s mcp (unat (get_waypoints_length s mcp))) i \<rbrace>
   LoadCode.MissionCommandUtils.FindWP' mcp i
-\<lbrace> \<lambda> r s. r = NULL \<and> P s\<rbrace>!"
- apply (unfold LoadCode.MissionCommandUtils.FindWP'_def)
- apply (simp add: skipE_def)
- apply(subst whileLoopE_add_inv[where M = "\<lambda> (j,s). unat (get_waypoints_length s mcp - j)"
-                                 and I = "\<lambda> j s. P s 
-\<and> is_valid_MissionCommand s mcp
-\<and> None = find_waypoint (lift_waypoints s mcp (unat (get_waypoints_length s mcp))) i
-"])
+\<lbrace> \<lambda> r s. P s \<and> r = NULL \<rbrace>!"
+  apply (unfold LoadCode.MissionCommandUtils.FindWP'_def)
+  apply (simp add: skipE_def)
+  apply(subst whileLoopE_add_inv
+        [where 
+          M = "\<lambda> (j,s). unat (get_waypoints_length s mcp - j)"
+          and I = "\<lambda> j s. P s 
+                          \<and> is_valid_MissionCommand s mcp
+                          \<and> None 
+                            = find_waypoint 
+                                (lift_waypoints s mcp (unat (get_waypoints_length s mcp))) 
+                                i"
+        ])
  apply wp
-   apply clarsimp
-   apply (metis find_waypoint_failure_not_equal_all_elems_aux get_waypoint_number_def is_valid_MissionCommand_def uint_nat word_less_nat_alt)
+    apply clarsimp
+    apply (metis find_waypoint_failure_all_neq_number get_waypoint_number_def 
+                 uint_nat word_less_nat_alt)
   apply simp
-  apply wp 
-  using is_valid_MissionCommand_def by blast
-
-lemma aux1:"None = find_waypoint (lift_waypoints s mcp (unat j)) i \<Longrightarrow>
-           j < get_waypoints_length s mcp \<Longrightarrow>
-           get_waypoint_number (get_waypoint s mcp (uint j)) = i \<Longrightarrow>
-           Some (get_waypoint s mcp (uint j)) = find_waypoint (lift_waypoints s mcp (unat (get_waypoints_length s mcp))) i"
-  by (metis find_waypoint_failure_not_equal_all_elems_aux find_waypoint_next_is_match get_waypoint_number_def not_None_eq uint_nat)
+  apply wp
+  using is_valid_MissionCommand_def by auto
     
 lemma findwp_to_funspec:
 "\<lbrace> \<lambda> (s::lifted_globals).
-  is_valid_MissionCommand s mcp \<and> P s\<rbrace>
+  P s
+  \<and> is_valid_MissionCommand s mcp\<rbrace>
   LoadCode.MissionCommandUtils.FindWP' mcp i
-\<lbrace> \<lambda> r s. P s \<and> (r = NULL \<and> None = find_waypoint (lift_waypoints s mcp (unat (get_waypoints_length s mcp))) i) 
-          \<or> ( r \<noteq> NULL \<and> is_valid_Waypoint_struct_C s r 
-              \<and> Some (heap_Waypoint_struct_C s r) = find_waypoint (lift_waypoints s mcp (unat (get_waypoints_length s mcp))) i) \<rbrace>!"
+\<lbrace> \<lambda> r s. 
+  P s 
+  \<and> r = NULL \<longrightarrow> None = find_waypoint (lift_waypoints s mcp (unat (get_waypoints_length s mcp))) i
+  \<and> r \<noteq> NULL 
+    \<longrightarrow> is_valid_Waypoint_struct_C s r 
+        \<and> Some (heap_Waypoint_struct_C s r) 
+          = find_waypoint (lift_waypoints s mcp (unat (get_waypoints_length s mcp))) i \<rbrace>!"
  apply (unfold LoadCode.MissionCommandUtils.FindWP'_def)
  apply (simp add: skipE_def)
- apply(subst whileLoopE_add_inv[where M = "\<lambda> (j,s). unat (get_waypoints_length s mcp - j)"
-                                 and I = 
-"\<lambda> j s. P s 
-\<and> is_valid_MissionCommand s mcp
-\<and> None = find_waypoint (lift_waypoints s mcp (unat j)) i
-\<and> (get_waypoint_number (get_waypoint s mcp (uint j)) = i \<or> get_waypoint_number (get_waypoint s mcp (uint j)) \<noteq> i)
-\<and> j \<le> get_waypoints_length s mcp
-\<and> 0 \<le> unat j
-"])
-   apply wp+
-    apply (clarsimp)
-    apply (rule+,metis is_valid_MissionCommand_def uint_nat word_less_nat_alt)
-    apply rule
-       apply (metis is_valid_MissionCommand_def uint_nat word_less_nat_alt)
-         apply (intro aux1,simp+)
-     apply (metis is_valid_MissionCommand_def uint_nat word_less_nat_alt)
-    apply rule+
-    apply (metis find_waypoint_extend_failure get_waypoint_number_def)
-  using inc_le apply (rule,blast)
-    apply (metis is_valid_MissionCommand_def uint_nat word_less_nat_alt)
-   apply clarsimp
+ apply(subst whileLoopE_add_inv
+      [where 
+          M = "\<lambda> (j,s). unat (get_waypoints_length s mcp - j)"
+          and I = 
+            "\<lambda> j s. P s 
+             \<and> is_valid_MissionCommand s mcp
+             \<and> None = find_waypoint (lift_waypoints s mcp (unat j)) i
+             \<and> (get_waypoint_number (get_waypoint s mcp (uint j)) = i 
+                \<or> get_waypoint_number (get_waypoint s mcp (uint j)) \<noteq> i)
+             \<and> j \<le> get_waypoints_length s mcp"
+      ])
   apply wp
-  apply clarsimp
-    by (simp add: find_waypoint_def is_valid_MissionCommand_def)
+    apply clarsimp
+    apply (metis find_waypoint_extend_failure get_waypoint_number_def inc_le)
+    apply blast
+  apply wp
+  using find_waypoint_def is_valid_MissionCommand_def by auto
 end
